defined the ROS string type in Coq. This is an example of what has to be automatically generated from ROS .msg files, by reusing what roshask does for Haskell.
Will test that the hand written code, especially the extraction directives result in the expected Haskell extract.

src/shim/Haskell/RoshaskMsg.v
@@ -17,7 +17,7 @@ Definition TopicName : Type := string.
   *)
 Definition ROSStream (T:Type) := CoList T.
 
-Class RoshashMsgType (T:Type) :=
+Class ROSMsgType (T:Type) :=
   {    
    subscribe : TopicName -> Node (ROSStream T);
    publish : TopicName -> ROSStream T -> Node unit (*will be mapped to advertize in Roshask*)
