src/shim/Haskell/ROSStringMsg.v
@@ -1,0 +1,30 @@
+Require Import RoshaskMsg.
+Require Import String.
+Require Import ExtrHaskellString.
+
+
+Extraction Language Haskell.
+
+(** temporary example for generation of Coq types for ROS messages, 
+   and extraction to corresponding Haskell messages.*)
+Record ROS_StdMsg_String := mkString
+                              {__data:string}.
+
+Extract Inductive ROS_StdMsg_String => "ROS.Std_msgs.String.String"
+                                            [ "ROS.Std_msgs.String.String"].
+
+Extract Constant __data => "ROS.Std_msgs.String.__data".
+
+Require Import RoshaskNodeMonad.
+
+Axiom subscribe_ROS_StdMsg_String : TopicName -> Node (ROSStream ROS_StdMsg_String).
+Extract Constant  subscribe_ROS_StdMsg_String => "(Ros.ROSCoqUtil.subscribeCoList)".
+
+Axiom publish_ROS_StdMsg_String : TopicName -> ROSStream ROS_StdMsg_String -> Node unit.
+Extract Constant  publish_ROS_StdMsg_String => "(Ros.ROSCoqUtil.publishCoList)".
+
+Instance ROSMsgInstance_ROS_StdMsg_String : ROSMsgType ROS_StdMsg_String :=
+  Build_ROSMsgType _  subscribe_ROS_StdMsg_String  publish_ROS_StdMsg_String.
+
+
+
